Dodate formulacije

uidt_2024_seminarski/algebra/Algebra.thy
@@ -586,6 +586,36 @@ locale Group = Monoid G "(\<cdot>)" \<e> for G and op (infixl "\<cdot>" 100) and
   assumes inverse_law [intro]: "a \<in> G \<Longrightarrow> invertable a"
 begin
 
+fun inv :: "'a ⇒ 'a" where
+  "inv a = (SOME b. a \<cdot> b = \<e>)"
+
+
+(*mi19172_Nikolina_Pejovic_FORMULACIJA*)
+lemma right_cancel:
+  assumes "a \<cdot> x = b \<cdot> x" and "a ∈ G" and "b ∈ G" and "x ∈ G"
+  shows "a = b"
+  sorry
+
+(*mi19172_Nikolina_Pejovic_FORMULACIJA*)
+lemma left_cancel:
+  assumes "x \<cdot> a = x \<cdot> b" and "x ∈ G" and "a ∈ G" and "b ∈ G"
+  shows "a = b"
+  sorry
+
+(*mi19172_Nikolina_Pejovic_FORMULACIJA*)
+primrec pow :: "'a ⇒ nat ⇒ 'a" where
+  "pow g 0 = \<e>"
+| "pow g (Suc n) = g \<cdot> pow g n"
+
+(*mi19172_Nikolina_Pejovic_FORMULACIJA*)
+primrec inv_pow :: "'a ⇒ nat ⇒ 'a" where
+  "inv_pow g 0 = \<e>"
+| "inv_pow g (Suc n) = inv g \<cdot> inv_pow g n"
+
+(*mi19172_Nikolina_Pejovic_FORMULACIJA*)
+lemma pow_sum: "pow g n \<cdot> pow g m = pow g (n + m)" and "g ∈ G" and "n ∈ ℕ" and "m ∈ ℕ"
+  sorry
+
 (*mi18044_Aleksa_Kostur_FORMULACIJA*)
 lemma pow_pow:  "⟦g ∈ G; m ∈ Z; n ∈ Z⟧ ⟹ (g ^ n) ^ m = g ^ (n * m)"
 (*<*) sorry (*>*)
